Modifiers/Merge.dfy
@@ -7,6 +7,8 @@ module Modifiers.Merge {
   import opened Subcircuit
   import opened Utils
   import opened Eval
+  import opened Path
+  import opened Path2
 
   predicate ScufMapsCanMerge(mp1: ScufMap, mp2: ScufMap)
   {
@@ -63,8 +65,9 @@ module Modifiers.Merge {
   {
     var si1 := SI(si.inputs[..uf1.input_width], si.state[..uf1.state_width]);
     var si2 := SI(si.inputs[uf1.input_width..], si.state[uf1.state_width..]);
+    reveal UpdateFunction.Valid();
     var so1 := uf1.sf(si1);
-    var so2 := uf1.sf(si2);
+    var so2 := uf2.sf(si2);
     var so := SO(so1.outputs + so2.outputs, so1.state + so2.state);
     so
   }
@@ -77,10 +80,79 @@ module Modifiers.Merge {
     var input_width := uf1.input_width + uf2.input_width;
     var output_width := uf1.output_width + uf2.output_width;
     var state_width := uf1.state_width + uf2.state_width;
+    reveal UpdateFunction.Valid();
     UpdateFunction(
       input_width, output_width, state_width,
       (si: SI) requires |si.inputs| == input_width && |si.state| == state_width => MergeSF(uf1, uf2, si)
     )
+  }
+
+  //lemma MergeUpdateFunctionProperties(uf1: UpdateFunction, uf2: UpdateFunction)
+  //      EvalOk(MFLookup(s1, fi1, np));
+  //      EvalOk(MFLookup(s, fi, np));
+
+  lemma MergeF1Properties(c: Circuit, s1: Scuf, s2: Scuf, np: NP, fi: FI)
+    requires MergeRequirements(c, s1, s2)
+    requires np in s1.mp.outputs || np in StateINPs(s1.mp.state)
+    requires
+      var s := MergeScufsImpl(c, s1, s2);
+      FIValid(fi, s.mp.inputs, s.mp.state)
+    ensures
+      var s := MergeScufsImpl(c, s1, s2);
+      var fi1 := MergeFI1(c, s1, s2, fi);
+      && (MFLookup(s, fi, np) == MFLookup(s1, fi1, np))
+  {
+    reveal Seq.ToSet();
+    var s := MergeScufsImpl(c, s1, s2);
+    var si := s.mp.fi2si(fi);
+    var si1 := SI(si.inputs[..s1.uf.input_width], si.state[..s1.uf.state_width]);
+    var si2 := SI(si.inputs[s1.uf.input_width..], si.state[s1.uf.state_width..]);
+    reveal UpdateFunction.Valid();
+    reveal NPsInSc();
+    s1.mp.si2fi2si(si1);
+    s2.mp.si2fi2si(si2);
+    reveal SeqsToMap();
+    reveal MapMatchesSeqs();
+    reveal MapToSeq();
+  }
+
+  lemma MergeF2Properties(c: Circuit, s1: Scuf, s2: Scuf, np: NP, fi: FI)
+    requires MergeRequirements(c, s1, s2)
+    requires np in s2.mp.outputs || np in StateINPs(s2.mp.state)
+    requires
+      var s := MergeScufsImpl(c, s1, s2);
+      FIValid(fi, s.mp.inputs, s.mp.state)
+    ensures
+      var s := MergeScufsImpl(c, s1, s2);
+      var fi2 := MergeFI2(c, s1, s2, fi);
+      && (MFLookup(s, fi, np) == MFLookup(s2, fi2, np))
+  {
+    reveal Seq.ToSet();
+    var s := MergeScufsImpl(c, s1, s2);
+    var si := s.mp.fi2si(fi);
+    var si1 := SI(si.inputs[..s1.uf.input_width], si.state[..s1.uf.state_width]);
+    var si2 := SI(si.inputs[s1.uf.input_width..], si.state[s1.uf.state_width..]);
+    reveal UpdateFunction.Valid();
+    reveal NPsInSc();
+    s1.mp.si2fi2si(si1);
+    s2.mp.si2fi2si(si2);
+    reveal SeqsToMap();
+    reveal MapMatchesSeqs();
+    reveal MapToSeq();
+    var fi2 := MergeFI2(c, s1, s2, fi);
+    var so2 := s2.uf.sf(si2);
+    var fo2 := s2.mp.so2fo(so2);
+    var so := s.uf.sf(si);
+    var fo := s.mp.so2fo(so);
+    MergeFO1FO2Properties(c, s1, s2, fi);
+    if np in s2.mp.outputs {
+      assert MFLookup(s2, fi2, np) == fo2.outputs[np];
+      assert MFLookup(s, fi, np) == fo.outputs[np];
+    } else {
+      assert MFLookup(s2, fi2, np) == fo2.state[np.n];
+      assert MFLookup(s, fi, np) == fo.state[np.n];
+    }
+    assert (MFLookup(s, fi, np) == MFLookup(s2, fi2, np));
   }
 
   lemma ScufsNoIntersectionMapsCanMerge(c: Circuit, s1: Scuf, s2: Scuf)
@@ -90,44 +162,344 @@ module Modifiers.Merge {
     requires s1.sc !! s2.sc
     ensures ScufMapsCanMerge(s1.mp, s2.mp)
   {
+    FInputsInSc(c, s1);
+    FInputsInSc(c, s2);
+    FOutputsInSc(c, s1);
+    FOutputsInSc(c, s2);
+    reveal NPsInSc();
+    reveal Seq.ToSet();
+  }
+
+  ghost predicate MergeRequirements(c: Circuit, s1: Scuf, s2: Scuf)
+  {
+    && c.Valid()
+    && s1.Valid(c)
+    && s2.Valid(c)
+    && s1.sc !! s2.sc
+    && IsIsland(c, s1.sc)
+    && IsIsland(c, s2.sc)
   }
 
   lemma IslandScufsAllInputsAdd(c: Circuit, s1: Scuf, s2:Scuf)
-    requires c.Valid()
-    requires s1.Valid(c)
-    requires s2.Valid(c)
-    requires s1.sc !! s2.sc
-    requires IsIsland(c, s1.sc)
-    requires IsIsland(c, s2.sc)
+    requires MergeRequirements(c, s1, s2)
     ensures
       reveal ScValid();
       AllInputs(c, s1.sc + s2.sc) == AllInputs(c, s1.sc) + AllInputs(c, s2.sc)
   {
+    reveal UnconnInputs();
+    reveal ConnInputs();
+    reveal ScValid();
+    assert UnconnInputs(c, s1.sc + s2.sc) == UnconnInputs(c, s1.sc) + UnconnInputs(c, s2.sc);
+    IsIslandNoInputs(c, s1.sc);
+    IsIslandNoInputs(c, s2.sc);
+    assert ConnInputs(c, s1.sc + s2.sc) == ConnInputs(c, s1.sc) + ConnInputs(c, s2.sc) by {
+      assert ConnInputs(c, s1.sc + s2.sc) <= ConnInputs(c, s1.sc) + ConnInputs(c, s2.sc);
+      assert ConnInputs(c, s1.sc + s2.sc) >= ConnInputs(c, s1.sc) + ConnInputs(c, s2.sc) by {
+      }
+    }
+  }
+
+  lemma MergeFICircuitValid(c: Circuit, s1: Scuf, s2: Scuf, np: NP, fi: FI)
+    requires MergeRequirements(c, s1, s2)
+    requires np in s1.mp.outputs || np in s2.mp.outputs ||
+             np in StateINPs(s1.mp.state) || np in StateINPs(s2.mp.state)
+    requires
+      var s := MergeScufsImpl(c, s1, s2);
+      FIValid(fi, s.mp.inputs, s.mp.state)
+    ensures
+      var s := MergeScufsImpl(c, s1, s2);
+      assert NPValid(c, np) by {
+        ScufFOutputsAreValid(c, s1);
+        ScufFOutputsAreValid(c, s2);
+      }
+      && FICircuitValid(c, fi)
+  {
+    reveal Seq.ToSet();
+    var s := MergeScufsImpl(c, s1, s2);
+    assert FICircuitValid(c, fi) by {
+      reveal Circuit.Valid();
+      ScufFInputsAreValid(c, s1);
+      ScufFInputsAreValid(c, s2);
+      assert s.mp.inputs == s1.mp.inputs + s2.mp.inputs;
+      assert forall np :: np in s.mp.inputs ==> INPValid(c, np);
+      assert (forall np :: np in fi.inputs.Keys ==> INPValid(c, np));
+      reveal AllSeq();
+      reveal ScValid();
+      reveal Scuf.SomewhatValid();
+      assert Seq.ToSet(s1.mp.state) == AllSeq(c, s1.sc);
+      assert Seq.ToSet(s2.mp.state) == AllSeq(c, s2.sc);
+      assert (forall n :: n in fi.state.Keys ==> n in c.NodeKind);
+      assert forall n :: n in AllSeq(c, s1.sc) ==> c.NodeKind[n].CSeq?;
+      assert forall n :: n in Seq.ToSet(s1.mp.state) ==> c.NodeKind[n].CSeq?;
+      assert forall n :: n in Seq.ToSet(s2.mp.state) ==> c.NodeKind[n].CSeq?;
+      assert forall n :: n in s1.mp.state ==> c.NodeKind[n].CSeq?;
+      assert forall n :: n in s2.mp.state ==> c.NodeKind[n].CSeq?;
+      assert (forall n :: n in fi.state.Keys ==> c.NodeKind[n].CSeq?);
+      reveal FICircuitValid();
+    }
+  }
+
+  function MergeFI1(c: Circuit, s1: Scuf, s2: Scuf, fi: FI): (fi1: FI)
+    requires MergeRequirements(c, s1, s2)
+    requires
+      var s := MergeScufsImpl(c, s1, s2);
+      FIValid(fi, s.mp.inputs, s.mp.state)
+  {
+    var s := MergeScufsImpl(c, s1, s2);
+    var si := s.mp.fi2si(fi);
+    var si1 := SI(si.inputs[..s1.uf.input_width], si.state[..s1.uf.state_width]);
+    var fi1 := s1.mp.si2fi(si1);
+    fi1
+  }
+
+  function MergeFI2(c: Circuit, s1: Scuf, s2: Scuf, fi: FI): (fi1: FI)
+    requires MergeRequirements(c, s1, s2)
+    requires
+      var s := MergeScufsImpl(c, s1, s2);
+      FIValid(fi, s.mp.inputs, s.mp.state)
+  {
+    var s := MergeScufsImpl(c, s1, s2);
+    var si := s.mp.fi2si(fi);
+    var si2 := SI(si.inputs[s1.uf.input_width..], si.state[s1.uf.state_width..]);
+    var fi2 := s2.mp.si2fi(si2);
+    fi2
+  }
+
+  function MergeFO1(c: Circuit, s1: Scuf, s2: Scuf, fi: FI): (fo1: FO)
+    requires MergeRequirements(c, s1, s2)
+    requires
+      var s := MergeScufsImpl(c, s1, s2);
+      FIValid(fi, s.mp.inputs, s.mp.state)
+  {
+    var s := MergeScufsImpl(c, s1, s2);
+    var si := s.mp.fi2si(fi);
+    var si1 := SI(si.inputs[..s1.uf.input_width], si.state[..s1.uf.state_width]);
+    reveal UpdateFunction.Valid();
+    var so1 := s1.uf.sf(si1);
+    var fo1 := s1.mp.so2fo(so1);
+    fo1
+  }
+
+  function MergeFO2(c: Circuit, s1: Scuf, s2: Scuf, fi: FI): (fo2: FO)
+    requires MergeRequirements(c, s1, s2)
+    requires
+      var s := MergeScufsImpl(c, s1, s2);
+      FIValid(fi, s.mp.inputs, s.mp.state)
+  {
+    var s := MergeScufsImpl(c, s1, s2);
+    var si := s.mp.fi2si(fi);
+    var si2 := SI(si.inputs[s1.uf.input_width..], si.state[s1.uf.state_width..]);
+    reveal UpdateFunction.Valid();
+    var so2 := s2.uf.sf(si2);
+    var fo2 := s2.mp.so2fo(so2);
+    fo2
+  }
+
+  function MergeFO(c: Circuit, s1: Scuf, s2: Scuf, fi: FI): (fo: FO)
+    requires MergeRequirements(c, s1, s2)
+    requires
+      var s := MergeScufsImpl(c, s1, s2);
+      FIValid(fi, s.mp.inputs, s.mp.state)
+  {
+    var s := MergeScufsImpl(c, s1, s2);
+    var si := s.mp.fi2si(fi);
+    var so := s.uf.sf(si);
+    var fo := s.mp.so2fo(so);
+    fo
+  }
+
+  lemma MergeFI1FI2Properties(c: Circuit, s1: Scuf, s2: Scuf, fi: FI)
+    requires MergeRequirements(c, s1, s2)
+    requires
+      var s := MergeScufsImpl(c, s1, s2);
+      FIValid(fi, s.mp.inputs, s.mp.state)
+    ensures
+      var fi1 := MergeFI1(c, s1, s2, fi);
+      var fi2 := MergeFI2(c, s1, s2, fi);
+      && fi.inputs == fi1.inputs + fi2.inputs
+      && fi.state == fi1.state + fi2.state
+  {
+    var s := MergeScufsImpl(c, s1, s2);
+    var si := s.mp.fi2si(fi);
+    var si1 := SI(si.inputs[..s1.uf.input_width], si.state[..s1.uf.state_width]);
+    var si2 := SI(si.inputs[s1.uf.input_width..], si.state[s1.uf.state_width..]);
+    assert si.inputs == si1.inputs + si2.inputs;
+    assert si.state == si1.state + si2.state;
+    var fi1 := s1.mp.si2fi(si1);
+    var fi2 := s2.mp.si2fi(si2);
+    reveal SeqsToMap();
+    assert Seq.ToSet(s1.mp.inputs) !! Seq.ToSet(s2.mp.inputs) by {
+      FInputsInSc(c, s1);
+      FInputsInSc(c, s2);
+      reveal NPsInSc();
+    }
+    SeqsToMapAdd(s1.mp.inputs, si1.inputs, s2.mp.inputs, si2.inputs);
+    SeqsToMapAdd(s1.mp.state, si1.state, s2.mp.state, si2.state);
+    s.mp.fi2si2fi(fi);
+  }
+
+  lemma MergeFO1FO2Properties(c: Circuit, s1: Scuf, s2: Scuf, fi: FI)
+    requires MergeRequirements(c, s1, s2)
+    requires
+      var s := MergeScufsImpl(c, s1, s2);
+      FIValid(fi, s.mp.inputs, s.mp.state)
+    ensures
+      var fo1 := MergeFO1(c, s1, s2, fi);
+      var fo2 := MergeFO2(c, s1, s2, fi);
+      var fo := MergeFO(c, s1, s2, fi);
+      && fo.outputs == fo1.outputs + fo2.outputs
+      && fo.state == fo1.state + fo2.state
+  {
+    var s := MergeScufsImpl(c, s1, s2);
+    var si := s.mp.fi2si(fi);
+    var so := s.uf.sf(si);
+    var si1 := SI(si.inputs[..s1.uf.input_width], si.state[..s1.uf.state_width]);
+    var si2 := SI(si.inputs[s1.uf.input_width..], si.state[s1.uf.state_width..]);
+    reveal UpdateFunction.Valid();
+    var so1 := s1.uf.sf(si1);
+    var so2 := s2.uf.sf(si2);
+    assert so.outputs == so1.outputs + so2.outputs;
+    assert so.state == so1.state + so2.state;
+    var fo1 := s1.mp.so2fo(so1);
+    var fo2 := s2.mp.so2fo(so2);
+    reveal SeqsToMap();
+    assert Seq.ToSet(s1.mp.outputs) !! Seq.ToSet(s2.mp.outputs) by {
+      FOutputsInSc(c, s1);
+      FOutputsInSc(c, s2);
+      reveal NPsInSc();
+    }
+    SeqsToMapAdd(s1.mp.outputs, so1.outputs, s2.mp.outputs, so2.outputs);
+    SeqsToMapAdd(s1.mp.state, so1.state, s2.mp.state, so2.state);
+    s.mp.fi2si2fi(fi);
+  }
+
+  lemma MergeNoPathBetweenOutputsAndInputs(c: Circuit, s1: Scuf, s2: Scuf, np: NP)
+    requires MergeRequirements(c, s1, s2)
+    ensures
+      var s1_outputs := Seq.ToSet(s1.mp.outputs) + StateINPs(s1.mp.state);
+      var s2_inputs := Seq.ToSet(s2.mp.inputs) + StateONPs(s2.mp.state);
+      !PathExistsBetweenNPSets(c, s1_outputs, s2_inputs)
+  {
+    var s1_outputs := Seq.ToSet(s1.mp.outputs) + StateINPs(s1.mp.state);
+    var s2_inputs := Seq.ToSet(s2.mp.inputs) + StateONPs(s2.mp.state);
+    forall np_1: NP, np_2: NP | np_1 in s1_outputs && np_2 in s2_inputs
+      ensures !PathExists(c, np_1, np_2)
+    {
+      reveal ScValid();
+      FOutputsInSc(c, s1);
+      FOutputsInSc(c, s2);
+      reveal NPsInSc();
+      assert np_1.n in s1.sc;
+      assert np_2.n in s2.sc;
+      NoPathOutOfIsland(c, s1.sc, np_1, np_2);
+    }
+    reveal PathExists();
+    reveal PathExistsBetweenNPSets();
   }
 
   lemma MergeEvaluatesCorrectly(c: Circuit, s1: Scuf, s2: Scuf, np: NP, fi: FI)
-    requires c.Valid()
-    requires s1.Valid(c)
-    requires s2.Valid(c)
-    requires s1.sc !! s2.sc
-    requires IsIsland(c, s1.sc)
-    requires IsIsland(c, s2.sc)
+    requires MergeRequirements(c, s1, s2)
     requires np in s1.mp.outputs || np in s2.mp.outputs ||
              np in StateINPs(s1.mp.state) || np in StateINPs(s2.mp.state)
-    requires FICircuitValid(c, fi)
+    requires
+      var s := MergeScufsImpl(c, s1, s2);
+      FIValid(fi, s.mp.inputs, s.mp.state)
     ensures
       var s := MergeScufsImpl(c, s1, s2);
-      Evaluate(c, np, fi) == EvalOk(MFLookup(s, fi, np))
+      assert NPValid(c, np) by {
+        ScufFOutputsAreValid(c, s1);
+        ScufFOutputsAreValid(c, s2);
+      }
+      && FICircuitValid(c, fi)
+      && (Evaluate(c, np, fi) == EvalOk(MFLookup(s, fi, np)))
   {
+    reveal Seq.ToSet();
+    var s := MergeScufsImpl(c, s1, s2);
+    MergeFICircuitValid(c, s1, s2, np, fi);
+    var si := s.mp.fi2si(fi);
+    var si1 := SI(si.inputs[..s1.uf.input_width], si.state[..s1.uf.state_width]);
+    var si2 := SI(si.inputs[s1.uf.input_width..], si.state[s1.uf.state_width..]);
+    var fi1 := s1.mp.si2fi(si1);
+    var fi2 := s2.mp.si2fi(si2);
+    assert NPValid(c, np) by {
+      ScufFOutputsAreValid(c, s1);
+      ScufFOutputsAreValid(c, s2);
+    }
+    reveal s.EvaluatesCorrectly();
+    if np in s1.mp.outputs || np in StateINPs(s1.mp.state) {
+      ScufValidFiValidToFICircuitValid(c, s1, fi1);
+      assert Evaluate(c, np, fi1) == EvalOk(MFLookup(s1, fi1, np));
+    } else {
+      ScufValidFiValidToFICircuitValid(c, s2, fi2);
+      assert Evaluate(c, np, fi2) == EvalOk(MFLookup(s2, fi2, np));
+    }
+    // No paths from the output of one scuf to the input of the other.
+    MergeNoPathBetweenOutputsAndInputs(c, s1, s2, np);
+    MergeNoPathBetweenOutputsAndInputs(c, s2, s1, np);
+    assert fi.inputs.Keys == fi1.inputs.Keys + fi2.inputs.Keys;
+    assert fi1.inputs.Keys !! fi2.inputs.Keys by {
+      FInputsInSc(c, s1);
+      FInputsInSc(c, s2);
+      reveal NPsInSc();
+    }
+    MergeFI1FI2Properties(c, s1, s2, fi);
+    if np in s1.mp.outputs || np in StateINPs(s1.mp.state) {
+      var state_onps := StateONPsFromSet(fi2.state.Keys);
+      assert !PathExistsToNPSet(c, np, fi2.inputs.Keys) && !PathExistsToNPSet(c, np, state_onps) by {
+        var s1_outputs := Seq.ToSet(s1.mp.outputs) + StateINPs(s1.mp.state);
+        var s2_inputs := Seq.ToSet(s2.mp.inputs) + StateONPs(s2.mp.state);
+        reveal PathExistsToNPSet();
+        reveal PathExistsBetweenNPSets();
+        NoPathExistsBetweenNPSetsToToNPSet(c, s1_outputs, s2_inputs, np);
+        NoPathExistsToNPSubSet(c, np, s2_inputs, fi2.inputs.Keys);
+        NoPathExistsToNPSubSet(c, np, s2_inputs, StateONPsFromSet(fi2.state.Keys));
+      }
+      EvaluateReduceFI(c, np, fi, fi2.inputs.Keys, fi2.state.Keys);
+      assert fi1.inputs.Keys == fi.inputs.Keys - fi2.inputs.Keys;
+      assert forall x: NP :: x in fi1.inputs && x in fi.inputs ==> fi1.inputs[x] == fi.inputs[x];
+      assert fi1.inputs == fi.inputs - fi2.inputs.Keys;
+      assert fi1 == FI(fi.inputs - fi2.inputs.Keys, fi.state - fi2.state.Keys);
+      calc {
+        Evaluate(c, np, fi);
+        Evaluate(c, np, fi1);
+        EvalOk(MFLookup(s1, fi1, np));
+        {
+          MergeF1Properties(c, s1, s2, np, fi);
+        }
+        EvalOk(MFLookup(s, fi, np));
+      }
+    } else {
+      var state_onps := StateONPsFromSet(fi1.state.Keys);
+      assert !PathExistsToNPSet(c, np, fi1.inputs.Keys) && !PathExistsToNPSet(c, np, state_onps) by {
+        var s2_outputs := Seq.ToSet(s2.mp.outputs) + StateINPs(s2.mp.state);
+        var s1_inputs := Seq.ToSet(s1.mp.inputs) + StateONPs(s1.mp.state);
+        reveal PathExistsToNPSet();
+        reveal PathExistsBetweenNPSets();
+        NoPathExistsBetweenNPSetsToToNPSet(c, s2_outputs, s1_inputs, np);
+        NoPathExistsToNPSubSet(c, np, s1_inputs, fi1.inputs.Keys);
+        NoPathExistsToNPSubSet(c, np, s1_inputs, StateONPsFromSet(fi1.state.Keys));
+      }
+      EvaluateReduceFI(c, np, fi, fi1.inputs.Keys, fi1.state.Keys);
+      assert fi2.inputs.Keys == fi.inputs.Keys - fi1.inputs.Keys;
+      assert forall x: NP :: x in fi2.inputs && x in fi.inputs ==> fi2.inputs[x] == fi.inputs[x];
+      assert fi2.inputs == fi.inputs - fi1.inputs.Keys;
+      assert fi2 == FI(fi.inputs - fi1.inputs.Keys, fi.state - fi1.state.Keys);
+      calc {
+        Evaluate(c, np, fi);
+        Evaluate(c, np, fi2);
+        EvalOk(MFLookup(s2, fi2, np));
+        {
+          MergeF2Properties(c, s1, s2, np, fi);
+        }
+        EvalOk(MFLookup(s, fi, np));
+      }
+    }
+
   }
 
   function MergeScufsImpl(c: Circuit, s1: Scuf, s2: Scuf): (s: Scuf)
-    requires c.Valid()
-    requires s1.Valid(c)
-    requires s2.Valid(c)
-    requires s1.sc !! s2.sc
-    requires IsIsland(c, s1.sc)
-    requires IsIsland(c, s2.sc)
+    requires MergeRequirements(c, s1, s2)
+    ensures s.MapValid()
   {
     var sc := s1.sc + s2.sc;
     assert ScufMapsCanMerge(s1.mp, s2.mp) by {
@@ -136,16 +508,13 @@ module Modifiers.Merge {
     var mp := MergeScufMaps(s1.mp, s2.mp);
     var uf := MergeUpdateFunctions(s1.uf, s2.uf);
     var s := Scuf(sc, mp, uf);
+    reveal NPsInSc();
+    reveal Seq.ToSet();
     s
   }
 
   function MergeScufs(c: Circuit, s1: Scuf, s2: Scuf): (s: Scuf)
-    requires c.Valid()
-    requires s1.Valid(c)
-    requires s2.Valid(c)
-    requires s1.sc !! s2.sc
-    requires IsIsland(c, s1.sc)
-    requires IsIsland(c, s2.sc)
+    requires MergeRequirements(c, s1, s2)
     ensures s.Valid(c)
   {
     var s := MergeScufsImpl(c, s1, s2);
@@ -153,15 +522,7 @@ module Modifiers.Merge {
     var uf := s.uf;
     var sc := s.sc;
     assert s.Valid(c) by {
-      assert s.MapValid() by {
-        assert mp.Valid();
-        assert mp.InSc(sc) by {
-          reveal NPsInSc();
-          reveal Seq.ToSet();
-        }
-        assert uf.Valid();
-        assert ScufMapUpdateFunctionConsistent(mp, uf);
-      }
+      assert s.MapValid();
       assert ScValid(c, s.sc) by {
         reveal ScValid();
       }
