Path2.dfy
@@ -9,32 +9,34 @@ module Path2 {
   // Prove that if there are no paths from onp to inps then we can remove inps from fi with
   // no effect on the outcome.
 
-  lemma EvaluateReduceFI(c: Circuit, np: NP, fi: FI, removed: set<NP>)
+  lemma EvaluateReduceFI(c: Circuit, np: NP, fi: FI, removed_inputs: set<NP>, removed_state: set<CNode>)
     requires c.Valid()
     requires NPValid(c, np)
     requires FICircuitValid(c, fi)
-    requires !PathExistsToNPSet(c, np, removed)
+    requires !PathExistsToNPSet(c, np, removed_inputs)
+    requires !PathExistsToNPSet(c, np, StateONPsFromSet(removed_state))
     ensures
-      var reduced_fi := FI(fi.inputs - removed, fi.state);
+      var reduced_fi := FI(fi.inputs - removed_inputs, fi.state - removed_state);
       reveal FICircuitValid();
       Evaluate(c, np, fi) == Evaluate(c, np, reduced_fi)
   {
-    var reduced_fi := FI(fi.inputs - removed, fi.state);
+    var reduced_fi := FI(fi.inputs - removed_inputs, fi.state - removed_state);
     reveal FICircuitValid();
     if ONPValid(c, np) {
-      EvaluateONPReduceFI(c, np, fi, removed);
+      EvaluateONPReduceFI(c, np, fi, removed_inputs, removed_state);
     } else {
-      EvaluateINPReduceFI(c, np, fi, removed);
+      EvaluateINPReduceFI(c, np, fi, removed_inputs, removed_state);
     }
   }
 
-  lemma EvaluateONPReduceFI(c: Circuit, np: NP, fi: FI, removed: set<NP>)
+  lemma EvaluateONPReduceFI(c: Circuit, np: NP, fi: FI, removed_inputs: set<NP>, removed_state: set<CNode>)
     requires c.Valid()
     requires FICircuitValid(c, fi)
     requires ONPValid(c, np)
-    requires !PathExistsToNPSet(c, np, removed)
+    requires !PathExistsToNPSet(c, np, removed_inputs)
+    requires !PathExistsToNPSet(c, np, StateONPsFromSet(removed_state))
     ensures
-      var reduced_fi := FI(fi.inputs - removed, fi.state);
+      var reduced_fi := FI(fi.inputs - removed_inputs, fi.state - removed_state);
       reveal FICircuitValid();
       EvaluateONP(c, np, fi) == EvaluateONP(c, np, reduced_fi)
   {
@@ -44,16 +46,17 @@ module Path2 {
     reveal PathValid();
     var p := [np];
     assert PathValid(c, p);
-    EvaluateONPInnerReduceFI(c, p, fi, removed);
+    EvaluateONPInnerReduceFI(c, p, fi, removed_inputs, removed_state);
   }
 
-  lemma EvaluateINPReduceFI(c: Circuit, np: NP, fi: FI, removed: set<NP>)
+  lemma EvaluateINPReduceFI(c: Circuit, np: NP, fi: FI, removed_inputs: set<NP>, removed_state: set<CNode>)
     requires c.Valid()
     requires FICircuitValid(c, fi)
     requires INPValid(c, np)
-    requires !PathExistsToNPSet(c, np, removed)
+    requires !PathExistsToNPSet(c, np, removed_inputs)
+    requires !PathExistsToNPSet(c, np, StateONPsFromSet(removed_state))
     ensures
-      var reduced_fi := FI(fi.inputs - removed, fi.state);
+      var reduced_fi := FI(fi.inputs - removed_inputs, fi.state - removed_state);
       reveal FICircuitValid();
       EvaluateINP(c, np, fi) == EvaluateINP(c, np, reduced_fi)
   {
@@ -61,26 +64,37 @@ module Path2 {
     var path := [np];
     LengthOneNoDuplicates(path);
     reveal PathValid();
-    EvaluateINPInnerReduceFI(c, path, fi, removed);
+    EvaluateINPInnerReduceFI(c, path, fi, removed_inputs, removed_state);
   }
 
-  lemma EvaluateONPInnerReduceFI(c: Circuit, p: seq<NP>, fi: FI, removed: set<NP>)
+  lemma EvaluateONPInnerReduceFI(c: Circuit, p: seq<NP>, fi: FI, removed_inputs: set<NP>, removed_state: set<CNode>)
     requires c.Valid()
     requires PathValid(c, p)
     requires EvaluateONPInnerRequirements(c, p, fi)
-    requires !PathExistsToNPSet(c, Seq.Last(p), removed)
+    requires !PathExistsToNPSet(c, Seq.Last(p), removed_inputs)
+    requires !PathExistsToNPSet(c, Seq.Last(p), StateONPsFromSet(removed_state))
     ensures
-      var reduced_fi := FI(fi.inputs - removed, fi.state);
+      var reduced_fi := FI(fi.inputs - removed_inputs, fi.state - removed_state);
       reveal FICircuitValid();
       EvaluateONPInner(c, p, fi) == EvaluateONPInner(c, p, reduced_fi)
     decreases |NodesNotInPath(c, p)|, 4
   {
-    var reduced_fi := FI(fi.inputs - removed, fi.state);
+    var reduced_fi := FI(fi.inputs - removed_inputs, fi.state - removed_state);
     reveal FICircuitValid();
     var head := Seq.Last(p);
     var nk := c.NodeKind[head.n];
     if head.n in fi.state {
-      assert head.n in reduced_fi.state;
+      assert head.n in reduced_fi.state by {
+        // The head can't be in the removed_state because we know there is no path to there.
+        if head.n !in reduced_fi.state {
+          assert head.n in removed_state;
+          assert head in StateONPsFromSet(removed_state);
+          reveal PathValid();
+          reveal PathExistsToNPSet();
+          assert PathToNPSet(c, [head], head, StateONPsFromSet(removed_state));
+          assert false;
+        }
+      }
       assert nk.CSeq? by {
         reveal FICircuitValid();
       }
@@ -90,10 +104,10 @@ module Path2 {
         }
     } else {
       match nk
-        case CXor() => EvaluateONPBinaryReduceFI(c, p, fi, removed);
-        case CAnd() => EvaluateONPBinaryReduceFI(c, p, fi, removed);
-        case CInv() => EvaluateONPUnaryReduceFI(c, p, fi, removed);
-        case CIden() => EvaluateONPUnaryReduceFI(c, p, fi, removed);
+        case CXor() => EvaluateONPBinaryReduceFI(c, p, fi, removed_inputs, removed_state);
+        case CAnd() => EvaluateONPBinaryReduceFI(c, p, fi, removed_inputs, removed_state);
+        case CInv() => EvaluateONPUnaryReduceFI(c, p, fi, removed_inputs, removed_state);
+        case CIden() => EvaluateONPUnaryReduceFI(c, p, fi, removed_inputs, removed_state);
         case CConst(b) => {
           reveal PathCaught();
         }
@@ -102,16 +116,17 @@ module Path2 {
     }
   }
 
-  lemma EvaluateONPBinaryReduceFI(c: Circuit, path: seq<NP>, fi: FI, removed: set<NP>)
+  lemma EvaluateONPBinaryReduceFI(c: Circuit, path: seq<NP>, fi: FI, removed_inputs: set<NP>, removed_state: set<CNode>)
     requires EvaluateONPBinaryRequirements(c, path, fi)
-    requires !PathExistsToNPSet(c, Seq.Last(path), removed)
+    requires !PathExistsToNPSet(c, Seq.Last(path), removed_inputs)
+    requires !PathExistsToNPSet(c, Seq.Last(path), StateONPsFromSet(removed_state))
     ensures
-      var reduced_fi := FI(fi.inputs - removed, fi.state);
+      var reduced_fi := FI(fi.inputs - removed_inputs, fi.state - removed_state);
       reveal FICircuitValid();
       EvaluateONPBinary(c, path, fi) == EvaluateONPBinary(c, path, reduced_fi)
     decreases |NodesNotInPath(c, path)|, 3
   {
-    var reduced_fi := FI(fi.inputs - removed, fi.state);
+    var reduced_fi := FI(fi.inputs - removed_inputs, fi.state - removed_state);
     reveal FICircuitValid();
     var nk := c.NodeKind[path[|path|-1].n];
     var head := Seq.Last(path);
@@ -130,23 +145,26 @@ module Path2 {
       assert |NodesNotInPath(c, path + [inp_0])| < |NodesNotInPath(c, path)|;
       StillHasNoDuplicates(path, inp_0);
       StillHasNoDuplicates(path, inp_1);
-      StillNoPathExistsToNPSet(c, Seq.Last(path), inp_0, removed);
-      StillNoPathExistsToNPSet(c, Seq.Last(path), inp_1, removed);
-      EvaluateINPInnerReduceFI(c, path + [inp_0], fi, removed);
-      EvaluateINPInnerReduceFI(c, path + [inp_1], fi, removed);
+      StillNoPathExistsToNPSet(c, Seq.Last(path), inp_0, removed_inputs);
+      StillNoPathExistsToNPSet(c, Seq.Last(path), inp_1, removed_inputs);
+      StillNoPathExistsToNPSet(c, Seq.Last(path), inp_0, StateONPsFromSet(removed_state));
+      StillNoPathExistsToNPSet(c, Seq.Last(path), inp_1, StateONPsFromSet(removed_state));
+      EvaluateINPInnerReduceFI(c, path + [inp_0], fi, removed_inputs, removed_state);
+      EvaluateINPInnerReduceFI(c, path + [inp_1], fi, removed_inputs, removed_state);
     }
   }
 
-  lemma EvaluateONPUnaryReduceFI(c: Circuit, path: seq<NP>, fi: FI, removed: set<NP>)
+  lemma EvaluateONPUnaryReduceFI(c: Circuit, path: seq<NP>, fi: FI, removed_inputs: set<NP>, removed_state: set<CNode>)
     requires EvaluateONPUnaryRequirements(c, path, fi)
-    requires !PathExistsToNPSet(c, Seq.Last(path), removed)
+    requires !PathExistsToNPSet(c, Seq.Last(path), removed_inputs)
+    requires !PathExistsToNPSet(c, Seq.Last(path), StateONPsFromSet(removed_state))
     ensures
-      var reduced_fi := FI(fi.inputs - removed, fi.state);
+      var reduced_fi := FI(fi.inputs - removed_inputs, fi.state - removed_state);
       reveal FICircuitValid();
       EvaluateONPUnary(c, path, fi) == EvaluateONPUnary(c, path, reduced_fi)
     decreases |NodesNotInPath(c, path)|, 3
   {
-    var reduced_fi := FI(fi.inputs - removed, fi.state);
+    var reduced_fi := FI(fi.inputs - removed_inputs, fi.state - removed_state);
     reveal FICircuitValid();
     var ending_set := fi.inputs.Keys + StateONPsFromSet(fi.state.Keys);
     var nk := c.NodeKind[path[|path|-1].n];
@@ -160,31 +178,33 @@ module Path2 {
       assert PathValid(c, new_path_0);
       assert |NodesNotInPath(c, path + [inp_0])| < |NodesNotInPath(c, path)|;
       StillHasNoDuplicates(path, inp_0);
-      StillNoPathExistsToNPSet(c, Seq.Last(path), inp_0, removed);
-      EvaluateINPInnerReduceFI(c, path + [inp_0], fi, removed);
+      StillNoPathExistsToNPSet(c, Seq.Last(path), inp_0, removed_inputs);
+      StillNoPathExistsToNPSet(c, Seq.Last(path), inp_0, StateONPsFromSet(removed_state));
+      EvaluateINPInnerReduceFI(c, path + [inp_0], fi, removed_inputs, removed_state);
     }
   }
 
-  lemma EvaluateINPInnerReduceFI(c: Circuit, path: seq<NP>, fi: FI, removed: set<NP>)
+  lemma EvaluateINPInnerReduceFI(c: Circuit, path: seq<NP>, fi: FI, removed_inputs: set<NP>, removed_state: set<CNode>)
     requires EvaluateINPInnerRequirements(c, path, fi)
-    requires !PathExistsToNPSet(c, Seq.Last(path), removed)
+    requires !PathExistsToNPSet(c, Seq.Last(path), removed_inputs)
+    requires !PathExistsToNPSet(c, Seq.Last(path), StateONPsFromSet(removed_state))
     ensures
-      var reduced_fi := FI(fi.inputs - removed, fi.state);
+      var reduced_fi := FI(fi.inputs - removed_inputs, fi.state - removed_state);
       reveal FICircuitValid();
       EvaluateINPInner(c, path, fi) == EvaluateINPInner(c, path, reduced_fi)
     decreases |NodesNotInPath(c, path)|, 2
   {
-    var reduced_fi := FI(fi.inputs - removed, fi.state);
+    var reduced_fi := FI(fi.inputs - removed_inputs, fi.state - removed_state);
     reveal FICircuitValid();
     var head := path[|path|-1];
     var tail := path[..|path|-1];
     if head in fi.inputs {
-      assert head !in removed by {
-        if head in removed {
+      assert head !in removed_inputs by {
+        if head in removed_inputs {
           reveal PathExistsToNPSet();
           var p_contradict := [head];
           reveal PathValid();
-          assert PathToNPSet(c, p_contradict, head, removed);
+          assert PathToNPSet(c, p_contradict, head, removed_inputs);
           assert false;
         }
       }
@@ -198,8 +218,9 @@ module Path2 {
           NodesNotInPathDecreases(c, path, onp);
           StillHasNoDuplicates(path, onp);
           AppendPathValid(c, path, onp);
-          StillNoPathExistsToNPSet(c, Seq.Last(path), onp, removed);
-          EvaluateONPInnerReduceFI(c, path + [onp], fi, removed);
+          StillNoPathExistsToNPSet(c, Seq.Last(path), onp, removed_inputs);
+          StillNoPathExistsToNPSet(c, Seq.Last(path), onp, StateONPsFromSet(removed_state));
+          EvaluateONPInnerReduceFI(c, path + [onp], fi, removed_inputs, removed_state);
           reveal PathCaught();
         }
       } else {
